avx2 absorb

proof/amd64/avx2/Keccak1600_fixedsizes_avx2.ec
@@ -22,12 +22,178 @@ from CryptoSpecs require import FIPS202_SHA3_Spec Keccakf1600_Spec Keccak1600_Sp
 require import Keccak1600_avx2 Keccakf1600_avx2.
 require import Keccak1600_subreadwrite.
 
+import IntOrder.
 
 
+op addstate_avx2 (s1: W256.t Array7.t, s2:state): W256.t Array7.t =
+ stavx2_from_st25 (addstate (stavx2_to_st25 s1) s2).
 
-(* TODO: to be moved elsewhere... *)
-op addstate_avx2 (st: W256.t Array7.t, l: W8.t list): W256.t Array7.t =
- stavx2_from_st25 (addstate (stavx2_to_st25 st) (bytes2state l)).
+op absorb_state_avx2 (st: W256.t Array7.t, l: W8.t list): W256.t Array7.t =
+ addstate_avx2 st (bytes2state l).
+
+op stavx2_pack w0 w1 w2 w3 w4 w5 w6 w7 w8 w9 =
+ sliceset256_64_25 
+  (sliceset256_64_25 
+   (sliceset256_64_25 
+    (sliceset256_64_25 
+     (sliceset256_64_25 (init_25_64 (fun i=>W64.zero)).[0 <- w0] (8*8) w1).[5 <- w2]
+     (8*48)
+     w3).[10 <- w4]
+    (8 * 88)
+    w5).[15 <- w6]
+   (8*128)
+   w7).[20 <- w8]
+  (8*168)
+  w9.
+
+
+op stavx2bytes_pack w0 w1 w2 w3 w4 w5 w6 w7 w8 w9 =
+u64bytes w0 ++ u256bytes w1 ++ u64bytes w2 ++
+ u256bytes w3 ++ u64bytes w4 ++ u256bytes w5 ++
+ u64bytes w6 ++ u256bytes w7 ++ u64bytes w8 ++
+ u256bytes w9.
+
+lemma stavx2_packE w0 w1 w2 w3 w4 w5 w6 w7 w8 w9:
+ stavx2_pack w0 w1 w2 w3 w4 w5 w6 w7 w8 w9
+ = bytes2state (stavx2bytes_pack w0 w1 w2 w3 w4 w5 w6 w7 w8 w9).
+proof.
+rewrite /bytes2state /Wpack /w64L_from_bytes /chunkify.
+have ->/=: size
+                (u64bytes w0 ++ u256bytes w1 ++ u64bytes w2 ++
+                 u256bytes w3 ++ u64bytes w4 ++ u256bytes w5 ++
+                 u64bytes w6 ++ u256bytes w7 ++ u64bytes w8 ++
+                 u256bytes w9) = 200.
+ by rewrite !size_cat !size_to_list.
+rewrite b2i0 /= /mkseq -iotaredE /stavx2bytes_pack /=.
+rewrite /u64bytes /u256bytes /= !W8u8.bits8E !W32u8.bits8E /pack8_t /=.
+by circuit.
+qed.
+
+phoare addstate_r3456_avx2_zero_ph _st:
+ [ M.__addstate_r3456_avx2
+ : st=_st /\ r3=W256.zero /\ r4=W256.zero /\ r5=W256.zero /\ r6=W256.zero
+ ==> res=_st
+ ] = 1%r.
+proof.
+proc; simplify.
+seq 1: #pre => //=.
+ by inline*; auto => />; circuit.
+by auto => />; circuit.
+by hoare; inline*; auto => />; circuit.
+qed.
+
+
+lemma stavx2INV_pabsorb r8 l st:
+ pabsorb_spec_avx2 r8 l st => stavx2INV st.
+proof.
+smt(stavx2INV_from_st25).
+qed.
+
+
+require import BitEncoding.
+import BitChunking.
+
+lemma chunk_take_eq' ['a] (n n': int) (l : 'a list):
+  0 < n => 
+  size l %/ n * n <= n' =>
+  chunk n l = chunk n (take n' l).
+proof.
+move => Hn Hn'; rewrite /chunk.
+have ->: size (take n' l) %/ n = size l %/ n.
+ rewrite size_take; first smt(size_ge0).
+ case: (n' < size l) => C //.
+ rewrite eqz_leq; split; last smt().
+ by apply leq_div2r; smt().
+apply eq_in_mkseq => i Hi /=.
+rewrite drop_take 1:/# take_take ifT //.
+have ?: i*n < size l by smt().
+have H1: n+i*n <= n'.
+ move: Hn'; rewrite -lez_divRL 1:/# => Hn'.
+ have H2: 1+i <= n' %/ n by smt(). 
+ apply (lez_trans (n' %/ n * n)); last smt().
+ by rewrite (:n+i*n=(1+i)*n) 1:/# ler_pmul2r /#.
+smt().
+qed.
+
+
+lemma drop_cat' ['a] (n : int) (s1 s2 : 'a list):
+ drop n (s1 ++ s2)
+ = if n <= size s1 then drop n s1 ++ s2 else drop (n - size s1) s2.
+proof.
+case: (n=size s1) => [->//=|C].
+ by rewrite drop_cat /= drop0 drop_size.
+by rewrite drop_cat /#.
+qed.
+
+lemma chunkremains_cat ['a] (l1 l2 : 'a list) (r : int):
+ 0 < r =>
+ chunkremains r (l1++l2) = chunkremains r (chunkremains r l1 ++ l2).
+proof.
+move=> Hr.
+rewrite /chunkremains size_cat eq_sym.
+rewrite drop_cat size_cat size_drop. smt(size_ge0).
+have ->: max 0 (size l1 - size l1 %/ r * r) = size l1 %% r by smt().
+rewrite drop_drop. smt(size_ge0). smt(size_ge0).
+case: ((size l1 %% r + size l2) %/ r * r < size l1 %% r) => C.
+ have E: (size l1 %% r + size l2) %/ r * r = 0 by smt(size_ge0).
+ rewrite E /= drop_cat' ifT.
+  by rewrite {1}(divz_eq (size l1) r) -addzA divzMDl 1:/# mulzDl E /= /#.
+ rewrite {2}(divz_eq (size l1) r) -addzA divzMDl 1:/# mulzDl E /= /#.
+rewrite drop_cat ifF.
+move: C; apply contra.
+  rewrite {1 2}(divz_eq (size l1) r) -addzA divzMDl 1:/#. smt().
+
+congr.
+rewrite eq_sym.
+rewrite {1}(divz_eq (size l1) r) -addzA divzMDl 1:/# mulzDl.
+rewrite {3}(divz_eq (size l1) r). ring.
+qed.
+
+lemma chunkremains_nil ['a] r (l: 'a list):
+ 0 < r =>
+ r %| size l =>
+ chunkremains r l = [].
+proof.
+by move=> Hr0 Hr; rewrite -size_eq0 size_chunkremains /#.
+qed.
+
+lemma bytes2state_cat l1 l2:
+ bytes2state (l1++l2)
+ = addstate (bytes2state l1) (bytes2state (u8zeros (size l1)++l2)).
+proof.
+rewrite -bytes2stbytesP.
+have: bytes2stbytes (l1 ++ l2)
+      = stbytes (addstate (bytes2state l1) (bytes2state (u8zeros (size l1) ++ l2))).
+ rewrite tP stbytes_addstate => i Hi.
+ rewrite /addstbytes map2iE // -!bytes2stbytesP !stwordsK !get_of_list // !nth_cat size_nseq ler_maxr.
+  smt(size_ge0).
+ case: (i < size l1) => C.
+  by rewrite nth_u8zeros.
+ by rewrite (nth_out _ l1) 1:/#.
+by move => ->; rewrite stbytesK.
+qed.
+ 
+lemma addstateC s1 s2:
+ addstate s1 s2 = addstate s2 s1.
+proof.
+rewrite tP => i Hi.
+by rewrite /addstate !initiE //= xorwC.
+qed.
+
+lemma chunk1 ['a] r (l: 'a list):
+ r <> 0 =>
+ size l = r =>
+ chunk r l = [l].
+proof.
+move=> Hr Hsz.
+by rewrite /chunk Hsz divzz Hr b2i1 mkseq1 /= drop0 -Hsz take_size.
+qed.
+
+lemma stateabsorb_iblocks_rcons l x st:
+ stateabsorb_iblocks (rcons l x) st
+ = keccak_f1600_op (stateabsorb (stateabsorb_iblocks l st) x).
+proof. by rewrite /stateabsorb_iblocks foldl_rcons /=. qed.
+
 
 
 
@@ -57,18 +223,6 @@ wp; call keccakf1600_avx2_ll.
 wp; call addstate_m_avx2_ll.
 by auto => /#.
 qed.
-
-require BitEncoding.
-import BitEncoding.BitChunking.
-
-(*
-op pabsorb_spec_avx2 (r8 : int) (l : W8.t list) (st : W256.t Array7.t) : bool =
-  0 < r8 <= 200 /\
-  st = stavx2_from_st25 
-        (addstate
-          (stateabsorb_iblocks (chunk r8 l) st0)
-          (bytes2state (chunkremains r8 l))).
-*)
 
 hoare absorb_m_avx2_h _mem _l _buf _len _r8 _tb:
  M.__absorb_m_avx2
@@ -193,6 +347,96 @@ clone import ReadWriteArray as RW
       theory WA <- WA
       proof _ASIZE_ge0 by exact _ASIZE_ge0
       proof _ASIZE_u64 by exact _ASIZE_u64.
+
+
+(* TODO: move/refactor this to somewhere else *)
+
+lemma take_to_list (buf: W8.t A.t) sz:
+ sz <= _ASIZE =>
+ take sz (A.to_list buf) = sub buf 0 sz.
+proof.
+move=> Hsz; case: (0 <= sz) => C.
+ by rewrite take_mkseq //.
+by rewrite take_le0 1:/# /sub mkseq0_le /#.
+qed.
+
+lemma drop_to_list (buf: W8.t A.t) sz:
+ 0 <= sz =>
+ drop sz (A.to_list buf) = sub buf sz (_ASIZE-sz).
+proof.
+move=> Hsz; case: (sz < _ASIZE) => C.
+ rewrite drop_mkseq 1:/#.
+ apply eq_mkseq => x.
+ by rewrite /(\o) /=.
+by rewrite drop_oversize ?size_to_list 1:/# /sub mkseq0_le 1:/#.
+qed.
+
+lemma chunk_cat_buf r8 l (buf: W8.t A.t):
+ let at = size l %% r8 in
+ let lastpos = (at + _ASIZE) %/ r8 * r8 - at in
+ 0 < r8 =>
+ chunk r8 (l ++ to_list buf)
+ = chunk r8 (l ++ sub buf 0 lastpos).
+proof.
+move=> /= H.
+rewrite !(chunk_cat' l) /= 1..2:/# /=; congr.
+rewrite chunk_take_eq 1:/# size_cat size_chunkremains size_to_list.
+rewrite take_cat' !size_chunkremains.
+case: (r8 <= size l %% r8 + _ASIZE) => C.
+ rewrite ifF 1:/#; congr; congr.
+ by rewrite take_to_list /#.
+rewrite divz_small /=; first smt(size_ge0 _ASIZE_ge0).
+rewrite ifT; first smt(size_ge0).
+rewrite take0 /sub mkseq0_le 1:/# cats0.
+by rewrite eq_sym chunk_take_eq 1:/# size_chunkremains divz_small 1:/# take0.
+qed.
+
+lemma sub0' (buf: W8.t A.t) off len:
+ len <= 0 =>
+ sub buf off len = [].
+proof. by move=> ?; rewrite /sub mkseq0_le. qed.
+
+lemma chunkremains_cat_buf r8 l (buf: W8.t A.t) tb:
+ let at = size l %% r8 in
+ let lastpos = (at + _ASIZE) %/ r8 * r8 - at in
+ let lastlen = if r8 <= at + _ASIZE then (at + _ASIZE) %% r8 else _ASIZE in
+ 0 < r8 =>
+ bytes2state (chunkremains r8 (l ++ to_list buf) ++ [tb])
+ = addstate
+    (bytes2state (chunkremains r8 (l ++ sub buf 0 lastpos)))
+    (bytes2state (u8zeros (if r8 <= size l %% r8 + _ASIZE then 0 else size l %% r8)
+                 ++ sub buf (_ASIZE - lastlen) lastlen ++ [tb])).
+proof.
+move=> at lastpos lastlen H.
+case: (r8 <= at + _ASIZE) => C.
+ rewrite eq_sym chunkremains_cat 1:/# eq_sym chunkremains_cat 1:/#.
+ rewrite /chunkremains !drop_cat !size_cat !size_to_list !size_sub 1:/#.
+ rewrite !size_drop; first smt(size_ge0).
+ rewrite ifF 1:/# ifF 1:/#.
+ have ->: (size l - size l %/ r8 * r8) = size l %% r8 by smt().
+ rewrite eq_sym drop_oversize 1:size_sub 1..2:/#.
+ rewrite nseq0_le 1:/# /=.
+ rewrite drop_to_list 1:/# bytes2state0 addstate_st0; congr; congr.
+ by rewrite /lastlen C /= ler_maxr /#. 
+rewrite {1}/A.sub mkseq0_le 1:/# cats0.
+rewrite chunkremains_cat 1:// chunkremains_small.
+ by rewrite size_cat size_chunkremains size_to_list /#.
+rewrite -!catA bytes2state_cat; congr; congr; congr.
+ by rewrite size_chunkremains /#. 
+rewrite /to_list /sub /=; congr; smt().
+qed.
+
+lemma sub_split len' (buf: W8.t A.t) off len:
+ 0 <= len' <= len =>
+ sub buf off len = sub buf off len' ++ sub buf (off+len') (len-len').
+proof.
+move=> Hlen.
+rewrite (:len=len'+(len-len')) 1:/# /sub mkseq_add 1..2:/#; congr.
+rewrite (:len' + (len - len') - len'=len-len') 1:/#.
+by apply eq_mkseq => i /= /#.
+qed.
+
+(* end TODO *)
 
 
 module MM = {
@@ -534,295 +778,8 @@ module MM = {
 
 module MMaux = {
   proc __addstate_avx2_aux (st:W256.t Array7.t, aT:int, buf:W8.t A.t,
-                        offset:int, _LEN:int, _TRAILB:int) : W256.t Array7.t *
-                                                             int * int = {
-    var dELTA:int;
-    var t64_1:W64.t;
-    var t128_0:W128.t;
-    var r0:W256.t;
-    var r1:W256.t;
-    var t64_2:W64.t;
-    var t128_1:W128.t;
-    var t128_2:W128.t;
-    var r3:W256.t;
-    var t64_3:W64.t;
-    var r4:W256.t;
-    var t64_4:W64.t;
-    var r5:W256.t;
-    var t64_5:W64.t;
-    var r6:W256.t;
-    var r2:W256.t;
-    t64_1 <- W64.zero;
-    r0 <- W256.zero;
-    r1 <- W256.zero;
-    t64_2 <- W64.zero;
-    t64_3 <- W64.zero;
-    t64_4 <- W64.zero;
-    t64_5 <- W64.zero;
-    r2 <- W256.zero;
-    r3 <- W256.zero;
-    r4 <- W256.zero;
-    r5 <- W256.zero;
-    r6 <- W256.zero;
-    dELTA <- 0;
-    if ((aT < 8)) {
-      if (((aT = 0) /\ (8 <= _LEN))) {
-        r0 <-
-        (VPBROADCAST_4u64
-        (get64_direct (WA.init8 (fun i => buf.[i]))
-        (W64.to_uint ((W64.of_int offset) + (W64.of_int dELTA)))));
-        dELTA <- (dELTA + 8);
-        _LEN <- (_LEN - 8);
-        aT <- 8;
-      } else {
-        (dELTA, _LEN, _TRAILB, aT, t64_1) <@ RW.MM.__a_ilen_read_upto8_at (
-        buf, offset, dELTA, _LEN, _TRAILB, 0, aT);
-        t128_0 <- (zeroextu128 t64_1);
-        r0 <- (VPBROADCAST_4u64 (truncateu64 t128_0));
-      }
-      st.[0] <- (st.[0] `^` r0);
-    } else {
-      
-    }
-    if (((aT < 40) /\ ((0 < _LEN) \/ (_TRAILB <> 0)))) {
-      (dELTA, _LEN, _TRAILB, aT, r1) <@ RW.MM.__a_ilen_read_upto32_at (buf, 
-      offset, dELTA, _LEN, _TRAILB, 8, aT);
-      st.[1] <- (st.[1] `^` r1);
-    } else {
-      
-    }
-    if (((0 < _LEN) \/ (_TRAILB <> 0))) {
-      (dELTA, _LEN, _TRAILB, aT, t64_2) <@ RW.MM.__a_ilen_read_upto8_at (buf,
-      offset, dELTA, _LEN, _TRAILB, 40, aT);
-      t128_1 <- (zeroextu128 t64_2);
-      t128_2 <- (set0_128);
-      if (((0 < _LEN) \/ (_TRAILB <> 0))) {
-        (dELTA, _LEN, _TRAILB, aT, r3) <@ RW.MM.__a_ilen_read_upto32_at (buf,
-        offset, dELTA, _LEN, _TRAILB, 48, aT);
-        (dELTA, _LEN, _TRAILB, aT, t64_3) <@ RW.MM.__a_ilen_read_upto8_at (
-        buf, offset, dELTA, _LEN, _TRAILB, 80, aT);
-        t128_2 <- (zeroextu128 t64_3);
-        (dELTA, _LEN, _TRAILB, aT, r4) <@ RW.MM.__a_ilen_read_upto32_at (buf,
-        offset, dELTA, _LEN, _TRAILB, 88, aT);
-        (dELTA, _LEN, _TRAILB, aT, t64_4) <@ RW.MM.__a_ilen_read_upto8_at (
-        buf, offset, dELTA, _LEN, _TRAILB, 120, aT);
-        t128_1 <- (VPINSR_2u64 t128_1 t64_4 (W8.of_int 1));
-        (dELTA, _LEN, _TRAILB, aT, r5) <@ RW.MM.__a_ilen_read_upto32_at (buf,
-        offset, dELTA, _LEN, _TRAILB, 128, aT);
-        (dELTA, _LEN, _TRAILB, aT, t64_5) <@ RW.MM.__a_ilen_read_upto8_at (
-        buf, offset, dELTA, _LEN, _TRAILB, 160, aT);
-        t128_2 <- (VPINSR_2u64 t128_2 t64_5 (W8.of_int 1));
-        (dELTA, _LEN, _TRAILB, aT, r6) <@ RW.MM.__a_ilen_read_upto32_at (buf,
-        offset, dELTA, _LEN, _TRAILB, 168, aT);
-        st <@ M.__addstate_r3456_avx2 (st, r3, r4, r5, r6);
-      } else {
-        
-      }
-      r2 <-
-      (W256.of_int
-      (((W128.to_uint t128_2) %% (2 ^ 128)) +
-      ((2 ^ 128) * (W128.to_uint t128_1))));
-      st.[2] <- (st.[2] `^` r2);
-    } else {
-      
-    }
-    offset <- (offset + dELTA);
-    return (st, aT, offset);
-  }
-  proc __addstate_avx2_aux2 (st:W256.t Array7.t, aT:int, buf:W8.t A.t,
-                        offset:int, _LEN:int, _TRAILB:int) : W256.t Array7.t *
-                                                             int * int = {
-    var dELTA:int;
-    var t64_1:W64.t;
-    var t128_0:W128.t;
-    var r0:W256.t;
-    var r1:W256.t;
-    var t64_2:W64.t;
-    var t128_1:W128.t;
-    var t128_2:W128.t;
-    var r3:W256.t;
-    var t64_3:W64.t;
-    var r4:W256.t;
-    var t64_4:W64.t;
-    var r5:W256.t;
-    var t64_5:W64.t;
-    var r6:W256.t;
-    var r2:W256.t;
-    t64_1 <- W64.zero;
-    r0 <- W256.zero;
-    r1 <- W256.zero;
-    t64_2 <- W64.zero;
-    t64_3 <- W64.zero;
-    t64_4 <- W64.zero;
-    t64_5 <- W64.zero;
-    r2 <- W256.zero;
-    r3 <- W256.zero;
-    r4 <- W256.zero;
-    r5 <- W256.zero;
-    r6 <- W256.zero;
-    dELTA <- 0;
-    if ((aT < 8)) {
-      if (((aT = 0) /\ (8 <= _LEN))) {
-        r0 <-
-        (VPBROADCAST_4u64
-        (get64_direct (WA.init8 (fun i => buf.[i]))
-        (W64.to_uint ((W64.of_int offset) + (W64.of_int dELTA)))));
-        dELTA <- (dELTA + 8);
-        _LEN <- (_LEN - 8);
-        aT <- 8;
-      } else {
-        (dELTA, _LEN, _TRAILB, aT, t64_1) <@ RW.MM.__a_ilen_read_upto8_at (
-        buf, offset, dELTA, _LEN, _TRAILB, 0, aT);
-        t128_0 <- (zeroextu128 t64_1);
-        r0 <- (VPBROADCAST_4u64 (truncateu64 t128_0));
-      }
-    } else {
-      
-    }
-    if (((aT < 40) /\ ((0 < _LEN) \/ (_TRAILB <> 0)))) {
-      (dELTA, _LEN, _TRAILB, aT, r1) <@ RW.MM.__a_ilen_read_upto32_at (buf, 
-      offset, dELTA, _LEN, _TRAILB, 8, aT);
-    } else {
-      
-    }
-    if (((0 < _LEN) \/ (_TRAILB <> 0))) {
-      (dELTA, _LEN, _TRAILB, aT, t64_2) <@ RW.MM.__a_ilen_read_upto8_at (buf,
-      offset, dELTA, _LEN, _TRAILB, 40, aT);
-      t128_1 <- (zeroextu128 t64_2);
-      t128_2 <- (set0_128);
-      if (((0 < _LEN) \/ (_TRAILB <> 0))) {
-        (dELTA, _LEN, _TRAILB, aT, r3) <@ RW.MM.__a_ilen_read_upto32_at (buf,
-        offset, dELTA, _LEN, _TRAILB, 48, aT);
-        (dELTA, _LEN, _TRAILB, aT, t64_3) <@ RW.MM.__a_ilen_read_upto8_at (
-        buf, offset, dELTA, _LEN, _TRAILB, 80, aT);
-        t128_2 <- (zeroextu128 t64_3);
-        (dELTA, _LEN, _TRAILB, aT, r4) <@ RW.MM.__a_ilen_read_upto32_at (buf,
-        offset, dELTA, _LEN, _TRAILB, 88, aT);
-        (dELTA, _LEN, _TRAILB, aT, t64_4) <@ RW.MM.__a_ilen_read_upto8_at (
-        buf, offset, dELTA, _LEN, _TRAILB, 120, aT);
-        t128_1 <- (VPINSR_2u64 t128_1 t64_4 (W8.of_int 1));
-        (dELTA, _LEN, _TRAILB, aT, r5) <@ RW.MM.__a_ilen_read_upto32_at (buf,
-        offset, dELTA, _LEN, _TRAILB, 128, aT);
-        (dELTA, _LEN, _TRAILB, aT, t64_5) <@ RW.MM.__a_ilen_read_upto8_at (
-        buf, offset, dELTA, _LEN, _TRAILB, 160, aT);
-        t128_2 <- (VPINSR_2u64 t128_2 t64_5 (W8.of_int 1));
-        (dELTA, _LEN, _TRAILB, aT, r6) <@ RW.MM.__a_ilen_read_upto32_at (buf,
-        offset, dELTA, _LEN, _TRAILB, 168, aT);
-      } else {
-        
-      }
-      r2 <-
-      (W256.of_int
-      (((W128.to_uint t128_2) %% (2 ^ 128)) +
-      ((2 ^ 128) * (W128.to_uint t128_1))));
-    } else {
-      
-    }
-    st.[0] <- (st.[0] `^` r0);
-    st.[1] <- (st.[1] `^` r1);
-    st <@ M.__addstate_r3456_avx2 (st, r3, r4, r5, r6);
-    st.[2] <- (st.[2] `^` r2);
-    offset <- (offset + dELTA);
-    return (st, aT, offset);
-  }
-  proc __addstate_avx2_aux3 (st:W256.t Array7.t, aT:int, buf:W8.t A.t,
-                        offset:int, _LEN:int, _TRAILB:int) : W256.t Array7.t *
-                                                             int * int = {
-    var dELTA:int;
-    var t64_1:W64.t;
-    var t128_0:W128.t;
-    var r0:W256.t;
-    var r1:W256.t;
-    var t64_2:W64.t;
-    var t128_1:W128.t;
-    var t128_2:W128.t;
-    var r3:W256.t;
-    var t64_3:W64.t;
-    var r4:W256.t;
-    var t64_4:W64.t;
-    var r5:W256.t;
-    var t64_5:W64.t;
-    var r6:W256.t;
-    var r2:W256.t;
-    t64_1 <- W64.zero;
-    r0 <- W256.zero;
-    r1 <- W256.zero;
-    t64_2 <- W64.zero;
-    t64_3 <- W64.zero;
-    t64_4 <- W64.zero;
-    t64_5 <- W64.zero;
-    r2 <- W256.zero;
-    r3 <- W256.zero;
-    r4 <- W256.zero;
-    r5 <- W256.zero;
-    r6 <- W256.zero;
-    dELTA <- 0;
-    if ((aT < 8)) {
-      if (((aT = 0) /\ (8 <= _LEN))) {
-        r0 <-
-        (VPBROADCAST_4u64
-        (get64_direct (WA.init8 (fun i => buf.[i]))
-        (W64.to_uint ((W64.of_int offset) + (W64.of_int dELTA)))));
-        dELTA <- (dELTA + 8);
-        _LEN <- (_LEN - 8);
-        aT <- 8;
-      } else {
-        (dELTA, _LEN, _TRAILB, aT, t64_1) <@ RW.MM.__a_ilen_read_upto8_at (
-        buf, offset, dELTA, _LEN, _TRAILB, 0, aT);
-        t128_0 <- (zeroextu128 t64_1);
-        r0 <- (VPBROADCAST_4u64 (truncateu64 t128_0));
-      }
-    } else {
-      
-    }
-    if (((aT < 40) /\ ((0 < _LEN) \/ (_TRAILB <> 0)))) {
-      (dELTA, _LEN, _TRAILB, aT, r1) <@ RW.MM.__a_ilen_read_upto32_at (buf, 
-      offset, dELTA, _LEN, _TRAILB, 8, aT);
-    } else {
-      
-    }
-    if (((0 < _LEN) \/ (_TRAILB <> 0))) {
-      (dELTA, _LEN, _TRAILB, aT, t64_2) <@ RW.MM.__a_ilen_read_upto8_at (buf,
-      offset, dELTA, _LEN, _TRAILB, 40, aT);
-      if (((0 < _LEN) \/ (_TRAILB <> 0))) {
-        (dELTA, _LEN, _TRAILB, aT, r3) <@ RW.MM.__a_ilen_read_upto32_at (buf,
-        offset, dELTA, _LEN, _TRAILB, 48, aT);
-        (dELTA, _LEN, _TRAILB, aT, t64_3) <@ RW.MM.__a_ilen_read_upto8_at (
-        buf, offset, dELTA, _LEN, _TRAILB, 80, aT);
-        (dELTA, _LEN, _TRAILB, aT, r4) <@ RW.MM.__a_ilen_read_upto32_at (buf,
-        offset, dELTA, _LEN, _TRAILB, 88, aT);
-        (dELTA, _LEN, _TRAILB, aT, t64_4) <@ RW.MM.__a_ilen_read_upto8_at (
-        buf, offset, dELTA, _LEN, _TRAILB, 120, aT);
-        (dELTA, _LEN, _TRAILB, aT, r5) <@ RW.MM.__a_ilen_read_upto32_at (buf,
-        offset, dELTA, _LEN, _TRAILB, 128, aT);
-        (dELTA, _LEN, _TRAILB, aT, t64_5) <@ RW.MM.__a_ilen_read_upto8_at (
-        buf, offset, dELTA, _LEN, _TRAILB, 160, aT);
-        (dELTA, _LEN, _TRAILB, aT, r6) <@ RW.MM.__a_ilen_read_upto32_at (buf,
-        offset, dELTA, _LEN, _TRAILB, 168, aT);
-      } else {
-        
-      }
-    } else {
-      
-    }
-    st.[0] <- (st.[0] `^` r0);
-    st.[1] <- (st.[1] `^` r1);
-    st <@ M.__addstate_r3456_avx2 (st, r3, r4, r5, r6);
-    t128_1 <- (zeroextu128 t64_2);
-    t128_1 <- (VPINSR_2u64 t128_1 t64_4 (W8.of_int 1));
-    t128_2 <- (zeroextu128 t64_3);
-    t128_2 <- (VPINSR_2u64 t128_2 t64_5 (W8.of_int 1));
-    r2 <-
-      (W256.of_int
-      (((W128.to_uint t128_2) %% (2 ^ 128)) +
-      ((2 ^ 128) * (W128.to_uint t128_1))));
-    st.[2] <- (st.[2] `^` r2);
-    offset <- (offset + dELTA);
-    return (st, aT, offset);
-  }
-  proc __addstate_avx2_aux4 (st:W256.t Array7.t, aT:int, buf:W8.t A.t,
-                        offset:int, _LEN:int, _TRAILB:int) : W256.t Array7.t *
-                                                             int * int = {
+                            offset:int, _LEN:int, _TRAILB:int
+                           ) : W256.t Array7.t * int * int = {
     var dELTA:int;
     var t64_1:W64.t;
     var t128_0:W128.t;
@@ -906,190 +863,17 @@ module MMaux = {
 lemma addstate_avx2_ll: islossless MM.__addstate_avx2
  by islossless.
 
-
-
-
-lemma subread_specP N buf off dlt len trail cur at dlt' at' w':
- 0 <= N =>
- cur <= at =>
- subread_pre cur at len trail =>
- subread_spec N buf off dlt len trail cur at dlt' 0 0 at' w' =>
- at' = at + len + b2i (trail%%256<>0)
- /\
- dlt' = dlt + len
- /\
- bytes2state (nseq at W8.zero ++ sub buf (off+dlt) len ++ [W8.of_int trail])
- = bytes2state (nseq cur W8.zero++w').
-proof.
-move=> Hn Hcur Hpre Hspec.
-move: (Hpre) (Hspec Hn Hpre) => {Hspec} /> ???? H1 H2 H3 H4 H5 *.
-split; first smt().
-rewrite tP => i Hi.
-rewrite !initiE //= !nth_w64L_from_bytes 1..2:/#.
-congr; apply W8u8.Pack.ext_eq => k Hk.
-rewrite !get_of_list //.
-rewrite eq_sym !nth_take 1..4:/# !nth_drop 1..4:/# -catA nth_cat 1:size_nseq ?Eat.
-case: (8 * i + k < max 0 cur) => Ccur //.
- rewrite nth_cat ?size_nseq ifT 1:/#.
- by rewrite !nth_nseq_if /#.
-rewrite eq_sym nth_cat size_nseq /=.
-case: (8*i+k < max 0 at) => C1.
- by rewrite nth_nseq_if nth_wat /#.
-have ->: max 0 at = at by smt().
-have ->: max 0 cur = cur by smt().
-case: (len=0) => C2.
- by rewrite C2 nth_wat 1..2:/# sub0 /#.
-by rewrite nth_cat ifF 1:size_sub /#.
-qed.
-
-
-
-op addst_avx2 (st : W256.t Array7.t) (st25: W64.t Array25.t) =
- stavx2_from_st25 (addstate (stavx2_to_st25 st) st25).
-
-(*
-op stavx2_to_bits (stavx2: W256.t Array7.t) =
- flatten (map W256.w2bits (to_list stavx2)).
-
-lemma size_stavx2_to_bits stavx2:
- size (stavx2_to_bits stavx2) = 1792.
-admitted.
-*)
-
-(*
-lemma stavx2_to_bitsE stavx2:
- stavx2_to_bits stavx2 = flatten (map W256.w2bits (to_list stavx2)).
-proof.
-rewrite /stavx2_to_bits map_mkseq /mkseq -iotaredE /(\o) /= !flatten_cons /= flatten_nil cats0 !catA.
-rewrite /state2bits /w64L_to_bits map_mkseq  /mkseq -iotaredE /(\o) /= !flatten_cons /= flatten_nil cats0 !catA.
-admitted.
-*)
-
-(*
-op stavx2_from_bits bs =
- Array7.of_list W256.zero (map W256.bits2w (chunkify 256 bs)).
-
-lemma stavx2_from_bitsK bs:
- size bs = 1792 =>
- stavx2_to_bits (stavx2_from_bits bs) = bs.
-proof.
-admitted.
-
-lemma stavx2_to_bitsK st:
- stavx2_from_bits (stavx2_to_bits st) = st.
-proof.
-admitted.
-
-
-
-
-lemma flatten_states_aux llbytes (stavx2: W256.t Array7.t) l:
- size (flatten llbytes) = 200 =>
- l = List.map bytes_to_bits llbytes =>
- flatten (stavx2_to_bits stavx2 :: l)
- = stavx2_to_bits stavx2
-   ++ state2bits (bytes2state (flatten llbytes)).
-proof.
-move=> Hsz El.
-rewrite El flatten_cons; congr.
-rewrite -state2bytes2bits bytes2stateK //.
-by rewrite bytes_to_bits_flatten; congr.
-qed.
-
-lemma w256_to_bytes_to_bits w:
- bytes_to_bits (W32u8.to_list w) = w2bits w.
-admitted.
-
-lemma flatten_states st w1 w2 w3 w4 w5 w6 w7 w8 w9 w10:
- flatten
-  ( stavx2_to_bits st ::
-   [ W64.w2bits w1; W256.w2bits w2
-   ; W64.w2bits w3; W256.w2bits w4
-   ; W64.w2bits w5; W256.w2bits w6
-   ; W64.w2bits w7; W256.w2bits w8
-   ; W64.w2bits w9; W256.w2bits w10
-   ])
- = stavx2_to_bits st
-   ++ state2bits
-       (bytes2state (flatten [ u64_to_bytes w1; u256_to_bytes w2
-                             ; u64_to_bytes w3; u256_to_bytes w4
-                             ; u64_to_bytes w5; u256_to_bytes w6
-                             ; u64_to_bytes w7; u256_to_bytes w8
-                             ; u64_to_bytes w9; u256_to_bytes w10
-                             ])).
-proof.
-pose L:= u64_to_bytes _::_.
-rewrite (flatten_states_aux L); last done.
- rewrite /L !flatten_cons flatten_nil cats0 !size_cat.
- by rewrite !W8u8.size_to_list !W32u8.size_to_list.
-by rewrite /L /= !w64_to_bytes_to_bits !w256_to_bytes_to_bits.
-qed.
-
-(*
-stavx2_to_bits stavx2 = state2bits (stavx2_to_st25 stavx2)
-*)
-(* PARA INVOCAR LEMA
-[ u64_to_bytes t64_1; u256_to_bytes r1
-; u64_to_bytes t64_2; u256_to_bytes r3
-; u64_to_bytes t64_3; u256_to_bytes r4
-; u64_to_bytes t64_4; u256_to_bytes r5
-; u64_to_bytes t64_5; u256_to_bytes r6
-]
-*)
-*)
-
-
-
-(*
-clone import PolyArray as Array53 with
-        op size = 53.
-
-bind array Array53."_.[_]" Array53."_.[_<-_]" Array53.to_list Array53.of_list Array53.t 53.
-realize tolistP by done.
-realize get_setP by smt(Array53.get_setE). 
-realize eqP by smt(Array53.tP).
-realize get_out by smt(Array53.get_out).
-realize gt0_size by done.
-
-require import Avx2_extra.
-
-op split_states (inp : W64.t Array53.t ): W256.t Array7.t * W64.t Array25.t =
- ( init_7_256 (fun ii => u256_pack4 inp.[4*ii+0] inp.[4*ii+1] inp.[4*ii+2] inp.[4*ii+3])
- , init_25_64 (fun ii => inp.[28+ii])
- ).
-
-op F4 (inp : W64.t Array53.t ) : W256.t Array7.t =
- let (stavx2, st) = split_states inp in addst_avx2 stavx2 st.
-op P4 (inp : W64.t Array53.t ) : bool =
- stavx2INV (split_states inp).`1.
-*)
-op st_pack (_at _sz:int) w1 w2 w3 w4 w5 w6 w7 w8 w9 w10 =
- bytes2state (flatten [ u64_to_bytes w1; u256_to_bytes w2
-                      ; u64_to_bytes w3; u256_to_bytes w4
-                      ; u64_to_bytes w5; u256_to_bytes w6
-                      ; u64_to_bytes w7; u256_to_bytes w8
-                      ; u64_to_bytes w9; u256_to_bytes w10
-                      ]).
-
-phoare addstate_r3456_avx2_0_ph _st:
- [ M.__addstate_r3456_avx2
- : st=_st /\ r3=W256.zero /\ r3=W256.zero /\ r3=W256.zero /\ r3=W256.zero
- ==> res=_st
- ] = 1%r.
-admitted.
-
 equiv addstate_aux_eq:
- MM.__addstate_avx2 ~ MMaux.__addstate_avx2_aux4
+ MM.__addstate_avx2 ~ MMaux.__addstate_avx2_aux
  : ={arg} ==> ={res}.
 proc; simplify.
 swap {2} [16..18] -12.
 seq 2 6: (#pre /\ ={dELTA}).
  sp; if => //=.
-  admit.
+  wp; call a_ilen_read_bcast_upto8_at_eq; auto => /> &m ?.
+  by move => [r1' r2' r3' r4' r5'] [r1 r2 r3 r4 r5] />.
  auto => /> &m _.
- rewrite tP => i Hi; rewrite get_setE //.
- case: (i=0) => //.
- admit (* OK *).
+ by move: (st{m}) => _st; clear; circuit.
 swap {2} 13 -10.
 seq 1 3: (#pre); simplify.
  sp; if => //=; first by sim.
@@ -1106,45 +890,24 @@ sp; if => //=.
   swap {1} [7..9] 2.
   swap {1} 15 -7.
   by sim.
- wp; ecall {2} (addstate_r3456_avx2_0_ph st{2}).
- auto => />.
- admit (* OK *).
-wp; ecall {2} (addstate_r3456_avx2_0_ph st{2}).
+ wp; ecall {2} (addstate_r3456_avx2_zero_ph st{2}).
+ auto => /> &m *.
+ by move: (st{m}) (t64_2{m}) => _st _t64_2; clear; circuit.
+wp; ecall {2} (addstate_r3456_avx2_zero_ph st{2}).
 auto => /> &m *.
 rewrite tP => i Hi; rewrite get_setE //.
 case: (i=2) => //.
-admit (* OK *).
+by move => /> *; move: (st{m}) => _st; clear; circuit.
 qed.
 
-
-op stt_pack w0 w1 w2 w3 w4 w5 w6 w7 w8 w9 =
- sliceset256_64_25 
-  (sliceset256_64_25 
-   (sliceset256_64_25 
-    (sliceset256_64_25 
-     (sliceset256_64_25 (init_25_64 (fun i=>W64.zero)).[0 <- w0] (8*8) w1).[2 <- w2]
-     (8*48)
-     w3).[4 <- w4]
-    (8 * 88)
-    w5).[6 <- w6]
-   (8*128)
-   w7).[8 <- w8]
-  (8*168)
-  w9.
-
-print addst_avx2. 
-op addst (st1 st2: W64.t Array25.t) = init_25_64 (fun i => st1.[i] `^` st2.[i]).
-print addst_avx2.
-op addst_avx2_ st st25 = stavx2_from_st25 (addst (stavx2_to_st25 st) st25).
-
-hoare addstate_at_avx2_h _st _buf _off _len _tb _at:
+hoare addstate_avx2_h _st _buf _off _len _tb _at:
  MM.__addstate_avx2
  : st=_st /\ buf=_buf /\ offset=_off /\ _LEN=_len /\ _TRAILB=_tb /\ aT=_at
  /\ 0 <= _at <= _at+_len <= 200 - b2i (_tb<>0) 
  /\ 0<= offset /\ offset + _len <= _ASIZE /\ 0 <= _tb < 256
  /\  stavx2INV _st
  ==> let l = nseq _at W8.zero ++ sub _buf _off _len ++ [W8.of_int _tb]
-     in res.`1 = addst_avx2_ _st (bytes2state l)
+     in res.`1 = addstate_avx2 _st (bytes2state l)
      /\ res.`2 = _at + _len + b2i (_tb<>0)
      /\ res.`3 = _off + _len.
 proof.
@@ -1153,16 +916,16 @@ have ->:
  Pr[MM.__addstate_avx2(st{m'}, aT{m'}, buf{m'}, offset{m'}, _LEN{m'},
                           _TRAILB{m'}) @ &m' :
    ! (res.`1 =
-      addst_avx2_ st{m'}
+      addstate_avx2 st{m'}
         (bytes2state
            (nseq aT{m'} W8.zero ++ sub buf{m'} offset{m'} _LEN{m'} ++
             [W8.of_int _TRAILB{m'}])) /\
       res.`2 = aT{m'} + _LEN{m'} + b2i (_TRAILB{m'} <> 0) /\
       res.`3 = offset{m'} + _LEN{m'})]
- = Pr[MMaux.__addstate_avx2_aux4(st{m'}, aT{m'}, buf{m'}, offset{m'}, _LEN{m'},
-                              _TRAILB{m'}) @ &m' :
+ = Pr[MMaux.__addstate_avx2_aux( st{m'}, aT{m'}, buf{m'}, offset{m'}, _LEN{m'}
+                               , _TRAILB{m'}) @ &m' :
    ! (res.`1 =
-      addst_avx2_ st{m'}
+      addstate_avx2 st{m'}
         (bytes2state
            (nseq aT{m'} W8.zero ++ sub buf{m'} offset{m'} _LEN{m'} ++
             [W8.of_int _TRAILB{m'}])) /\
@@ -1178,32 +941,42 @@ byphoare (_: st=_st /\ buf=_buf /\ offset=_off /\ _LEN=_len /\ _TRAILB=_tb /\ aT
  /\  stavx2INV _st ==> _) => //; last by smt().
 hoare.
 clear; proc; simplify.
-pose _astate := (bytes2state (nseq _at W8.zero ++ sub _buf _off _len ++ [W8.of_int _tb])).
-seq 15: ( st=_st /\ _astate = stt_pack t64_1 r1 t64_2 r3 t64_3 r4 t64_4 r5 t64_5 r6 /\ aT = _at + _len + b2i (_tb <> 0) /\ offset = _off + _len /\ stavx2INV _st).
+pose _statebytes := nseq _at W8.zero ++ sub _buf _off _len ++ [W8.of_int _tb].
+seq 15: ( st=_st /\
+          bytes2state _statebytes = bytes2state (stavx2bytes_pack t64_1 r1 t64_2 r3 t64_3 r4 t64_4 r5 t64_5 r6)
+          /\ aT = _at + _len + b2i (_tb <> 0) /\ offset = _off + _len /\ stavx2INV _st).
  seq 3: ( #[1:3,8:]pre
         /\ subread_pre 0 _at _len _tb
-        /\ subread_spec 8 _buf _off 0 _len _tb 0 _at dELTA _LEN _TRAILB aT (u64_to_bytes t64_1)).
+        /\ subread_spec 8 _buf _off 0 _len _tb 0 _at dELTA _LEN _TRAILB aT (u64bytes t64_1)).
   case: (aT < 8).
    rcondt 3; first by auto.
-   admit.
+   ecall (a_ilen_read_upto8_at_h buf offset dELTA _LEN _TRAILB 0 aT).
+   by auto => &m /#.
   rcondf 3; first by auto.
-  auto => |>.
-  admit.
+  auto => |> *; split; first smt().
+  by apply subread_spec_ahead8 => /#.
  seq 2: ( #[/:-2]pre
-        /\ subread_spec 40 _buf _off 0 _len _tb 0 _at dELTA _LEN _TRAILB aT (u64_to_bytes t64_1++u256_to_bytes r1)).
+        /\ subread_spec 40 _buf _off 0 _len _tb 0 _at dELTA _LEN _TRAILB aT (u64bytes t64_1++u256bytes r1)).
   case: (aT < 40 /\ (0 < _LEN \/ _TRAILB <> 0)).
    rcondt 2; first by auto.
-   admit.
+   ecall (a_ilen_read_upto32_at_h buf offset dELTA _LEN _TRAILB 8 aT).
+   auto => |> &m ?????? H0 ? Hsz [dlt' len' tb' at' w'] /= H1.
+   by apply (subread_spec_cat _ _ _ _ _ _ _ _ _ _ _ _ _ _ _ _ _ _ _ _ _ H0 H1).
   rcondf 2; first by auto.
-  auto => |> &m.
-  admit.
+  auto => |> &m ?????? H0 /negb_and [Hat|Hsz].
+   have H1:= subread_spec_ahead32 _buf _off dELTA{m} _LEN{m} _TRAILB{m} 8 aT{m} _; first by smt().
+   by apply (subread_spec_cat _ _ _ _ _ _ _ _ _ _ _ _ _ _ _ _ _ _ _ _ _ H0 H1).
+  have H1:= subread_spec_empty32 _buf _off dELTA{m} _LEN{m} _TRAILB{m} 8 aT{m} _; first by smt().
+  by apply (subread_spec_cat _ _ _ _ _ _ _ _ _ _ _ _ _ _ _ _ _ _ _ _ _ H0 H1).
  case: (0 < _LEN \/ _TRAILB <> 0).
   rcondt 9; first by auto.
   swap [2..8] 1.
   seq 2: ( #[/:-3]pre
          /\ subread_spec 48 _buf _off 0 _len _tb 0 _at dELTA _LEN _TRAILB aT
-             (u64_to_bytes t64_1++u256_to_bytes r1++u64_to_bytes t64_2)).
-   admit.
+             (u64bytes t64_1++u256bytes r1++u64bytes t64_2)).
+   ecall (a_ilen_read_upto8_at_h buf offset dELTA _LEN _TRAILB 40 aT).
+   auto => |> &m ?????? H0 Hsz [dlt' len' tb' at' w'] /= H1.
+   by apply (subread_spec_cat _ _ _ _ _ _ _ _ _ _ _ _ _ _ _ _ _ _ _ _ _ H0 H1).
   sp; if => //=.
    wp; ecall (a_ilen_read_upto32_at_h buf offset dELTA _LEN _TRAILB 168 aT).
    ecall (a_ilen_read_upto8_at_h buf offset dELTA _LEN _TRAILB 160 aT).
@@ -1226,23 +999,29 @@ seq 15: ( st=_st /\ _astate = stt_pack t64_1 r1 t64_2 r3 t64_3 r4 t64_4 r5 t64_5
    have {H4 H2c} H2c:= (subread_spec_cat _ _ _ _ _ _ _ _ _ _ _ _ _ _ _ _ _ _ _ _ _ H4 H2c) => //.
    have {H2c H5} H5:= (subread_spec_cat _ _ _ _ _ _ _ _ _ _ _ _ _ _ _ _ _ _ _ _ _ H2c H5) => //.
    have {H5 H2d} H2d:= (subread_spec_cat _ _ _ _ _ _ _ _ _ _ _ _ _ _ _ _ _ _ _ _ _ H5 H2d) => //.
-   have {H2d H6} H6:= (subread_spec_cat _ _ _ _ _ _ _ _ _ _ _ _ _ _ _ _ _ _ _ _ _ H2d H6) => //.
-   have H:= subread_finish 200 _ _ _ _ _ _ _ _ _ _ _ _ _ _ _ H6 => //. 
-   admit.
-  auto => |> &m ????????.
-  admit (* st_pack... *).
+   have {H2d H6} /= H6:= (subread_spec_cat _ _ _ _ _ _ _ _ _ _ _ _ _ _ _ _ _ _ _ _ _ H2d H6) => //.
+   have := subread_full _ _ _ _ _ _ _ _ _ _ _ H6 _; first 2 smt().
+   by rewrite /= => />.
+  auto => |> &m ?????? H6 /negb_or [Hlen Htb].
+  have := subread_finished 48 _ _ _ _ _ _ _ _ _ _ _ _ H6 _ _; first 4 smt().
+  move=> [? [? ->]]; split; last smt().
+  rewrite /stavx2bytes_pack -!catA !u256bytes0 !u64bytes0 !cat_nseq //= !catA.
+  by rewrite bytes2state_zext.
  rcondf 9; first by auto.
- auto => |> &m ????????.
- admit (* st_pack... *).
+ auto => |> &m ?????? H6 ?.
+  split; last smt().
+  have := subread_finished 40 _ _ _ _ _ _ _ _ _ _ _ _ H6 _ _; first 4 smt().
+  move=> [? [? ->]]. 
+  rewrite /stavx2bytes_pack -!catA !u256bytes0 !u64bytes0 !cat_nseq //= !catA.
+  by rewrite bytes2state_zext.
 (* handling the permutation part with 'circuit' *)
-conseq (: st = _st /\ _astate = stt_pack t64_1 r1 t64_2 r3 t64_3 r4 t64_4 r5 t64_5 r6 /\ stavx2INV _st ==> st = addst_avx2_ _st _astate) => //=.
-inline *. 
-move: _astate _st => _astate _st; clear. 
-admit (* ??? anomaly: File "src/ecCircuits.ml", line 817, characters 2-8: Assertion failed
-circuit.
-*).
+exlim t64_1 => _t64_1; exlim r1 => _r1; exlim t64_2 => _t64_2; exlim r3 => _r3; exlim t64_3 => _t64_3; exlim r4 => _r4; exlim t64_4 => _t64_4; exlim r5 => _r5; exlim t64_5 => _t64_5; exlim r6 => _r6.
+move: _st => _st.
+conseq (: st = _st /\ stavx2INV _st /\ t64_1=_t64_1 /\ r1=_r1 /\ t64_2=_t64_2 /\ r3=_r3 /\ t64_3=_t64_3 /\ r4=_r4 /\ t64_4=_t64_4 /\ r5=_r5 /\ t64_5=_t64_5 /\ r6=_r6 ==> st = addstate_avx2 _st (stavx2_pack _t64_1 _r1 _t64_2 _r3 _t64_3 _r4 _t64_4 _r5 _t64_5 _r6)) => //=.
+ by rewrite /_astate stavx2_packE => /> * /#.
+inline *; clear.
+by circuit.
 qed.
-
 
 lemma absorb_avx2_ll: islossless MM.__absorb_avx2.
 proof.
@@ -1266,18 +1045,173 @@ hoare absorb_avx2_h _l _buf _tb _r8:
  MM.__absorb_avx2
  : aT = size _l %% _r8 /\ buf=_buf /\ _RATE8=_r8 /\ _TRAILB=_tb
  /\ pabsorb_spec_avx2 _r8 _l st
+ /\ 0 <= _tb < 256 
  ==> if _tb <> 0
      then absorb_spec_avx2 _r8 _tb (_l ++ to_list _buf) res.`1
      else pabsorb_spec_avx2 _r8 (_l ++ to_list _buf) res.`1
           /\ res.`2 = (size _l + _ASIZE) %% _r8.
 proof.
 proc => /=.
-admitted.
+have ?:= _ASIZE_u64.
+have ?:= _ASIZE_ge0.
+pose _at := size _l %% _r8.
+pose niters := (_at + _ASIZE) %/ _r8.
+pose lastlen := if _r8 <= _at + _ASIZE then (_at + _ASIZE) %% _r8 else _ASIZE.
+pose lastpos := niters * _r8 - _at.
+
+seq 3: (buf=_buf /\ _RATE8=_r8 /\ _TRAILB = _tb /\ 0 <= _tb < 256 
+       /\ pabsorb_spec_avx2 _r8 (_l ++ sub _buf 0 lastpos) st
+       /\ offset = _ASIZE - lastlen /\ _LEN = lastlen 
+       /\ aT = if _RATE8 <= _at + _ASIZE then 0 else _at).
+ sp; if => //; last first.
+  auto => |> *.
+  rewrite sub0' ?cats0.
+   by rewrite /lastpos /niters divz_small 1:/# /= /#.
+  smt().
+ wp; while ( buf=_buf /\ _RATE8 = _r8 /\ _TRAILB = _tb /\ 0 <= _tb < 256 /\ 
+             iTERS= (size _l %% _r8 + _ASIZE) %/ _r8 - 1 /\
+             offset = (i+1)*_r8 - size _l %% _r8 /\
+             0 <= i <= iTERS /\
+             pabsorb_spec_avx2 _r8 (_l ++ sub _buf 0 ((i+1)*_r8-size _l %% _r8)) st
+           ).
+  wp; ecall (keccakf1600_avx2_h (stavx2_to_st25 st)).
+  ecall (addstate_avx2_h st buf offset _RATE8 0 0).
+  auto => |> &m Htb0 Htb1 Hi0 Hi1.
+  rewrite {1}/pabsorb_spec_avx2 => [[Hr8]].
+  rewrite {1}/PABSORB1600 chunkremains_nil 1:/#.
+   rewrite size_cat size_sub 1:/# addzA (addzC (size _l)) -addzA.
+   rewrite {1}(divz_eq (size _l) _r8) -addzA /= -mulzDl dvdzP.
+   by exists (i{m} + 1 + size _l %/ _r8).
+  rewrite /stateabsorb bytes2state0 addstateC addstate_st0 => Est Hb.
+  rewrite !b2i0 /=; split.
+   split; first smt().
+   split; first smt().
+   split.
+    rewrite (:(i{m} + 1) * _r8 - size _l %% _r8 + _r8 <= _ASIZE
+             =(i{m}+2)*_r8<=size _l%%_r8+_ASIZE) 1:/#.
+    have Hb': i{m}+2 <= (size _l %% _r8 + _ASIZE) %/ _r8 by smt().
+    apply (ler_trans ((size _l %% _r8 + _ASIZE) %/ _r8 * _r8)).
+     by apply ler_wpmul2r; smt().
+    by apply lez_floor; smt().
+   by rewrite Est stavx2INV_from_st25.
+  move => Hr80 Hr81 He0 He1 Hst [st' at' len'] /= Est' _ Elen'; split.
+   by rewrite stavx2_to_st25K // Est' stavx2INV_from_st25.
+  move => _; split; first smt().
+  split; first smt().
+  split; first smt().
+  congr; rewrite /PABSORB1600 chunkremains_nil 1:/#.
+   rewrite size_cat size_sub 1:/# addzA (addzC (size _l)) -addzA.
+   rewrite {1}(divz_eq (size _l) _r8) -addzA /= -mulzDl dvdzP.
+   by exists (i{m} + 2 + size _l %/ _r8).
+  rewrite /stateabsorb bytes2state0 addstateC addstate_st0.
+  rewrite (sub_split ((i{m} + 1) * _r8 - size _l %% _r8)) 1:/# catA chunk_cat /=.
+   rewrite size_cat size_sub 1:/# addzA (addzC (size _l)) -addzA.
+   rewrite {1}(divz_eq (size _l) _r8) -addzA /= -mulzDl dvdzP.
+   by exists (i{m} + 1 + size _l %/ _r8).
+  rewrite (chunk1 _ (sub _buf _ _)) 1:/#.
+   by rewrite size_sub /#.
+  rewrite cats1 stateabsorb_iblocks_rcons Est' stavx2_from_st25K /stateabsorb; congr; congr.
+   by rewrite Est stavx2_from_st25K.
+  by rewrite nseq0 /= -(nseq1 W8.zero) bytes2state_zext; congr; congr; smt().
+ wp; ecall (keccakf1600_avx2_h (stavx2_to_st25 st)).
+ wp; ecall (addstate_avx2_h st buf offset (_RATE8 - aT) 0 aT).
+ auto => |> &m.
+ rewrite /pabsorb_spec_avx2 /PABSORB1600 /stateabsorb => [[Hr8]] Est ?? Hc.
+ split.
+  split; first smt().
+  split; first smt().
+  by rewrite Est stavx2INV_from_st25.
+ move=> |> ????? [st' at' len'] /=.
+ rewrite !b2i0 /= => Est' _ _; split.
+  by rewrite stavx2_to_st25K Est' // /addstate_avx2; apply stavx2INV_from_st25.
+ move=> _; split.
+  split.
+   by rewrite (:_ASIZE - (_r8 - size _l %% _r8) = size _l %% _r8 + _ASIZE + (-1)*_r8) 1:/# divzMDr /#.
+  split; first smt().
+  rewrite chunkremains_nil 1:/#.
+   rewrite size_cat size_sub 1:/# addzA (addzC (size _l)) -addzA.
+   rewrite {1}(divz_eq (size _l) _r8) -addzA /= -{2}(mul1z _r8) -mulzDl dvdzP.
+   by exists (1 + size _l %/ _r8).
+  rewrite /stateabsorb bytes2state0 addstateC addstate_st0; congr.
+  rewrite chunk_cat' 1:/# (chunk1 _ (_++_)) 1:/#.
+   by rewrite size_cat size_chunkremains size_sub /#.
+  rewrite cats1 stateabsorb_iblocks_rcons Est' Est !stavx2_from_st25K /stateabsorb. 
+  rewrite -addstateA; congr; congr.
+  rewrite -(nseq1 W8.zero) bytes2state_zext eq_sym bytes2state_cat; congr; congr.
+  by rewrite size_chunkremains.
+ move => i ??????.
+ have ->: i=(_ASIZE - (_r8 - size _l %% _r8)) %/ _r8 by smt().
+ have E: (_ASIZE - (_r8 - size _l %% _r8))%/_r8 = (size _l %% _r8 + _ASIZE)%/_r8 - 1.
+  have ->: _ASIZE - (_r8 - size _l %% _r8) = (size _l %% _r8 + _ASIZE + (-1)*_r8) by smt().
+  by rewrite divzMDr /#.
+ split.
+  congr; congr; congr; congr; congr; congr.
+   by rewrite /lastpos /niters /_at E /=.
+  by rewrite /lastpos /niters /_at E /=.
+ split.
+  by rewrite /lastlen ifT 1:/# /_at E /= /#. 
+ split.
+  rewrite /lastlen ifT 1:/# /_at.
+  by rewrite (:_ASIZE - (_r8 - size _l %% _r8) = _ASIZE + size _l %% _r8 + (-1)*_r8) 1:/# modzMDr /#.
+ by rewrite ifT /#.
+
+case: (_TRAILB<>0).
+ rcondt 2; first by call (:true ==> true) => //.
+ ecall (addratebit_avx2_h _RATE8 st).
+ ecall (addstate_avx2_h st buf offset _LEN _TRAILB aT).
+ auto => |> &m ?? H *.
+ split.
+  split; first smt(). 
+  split; rewrite /lastlen.
+   case: (_r8 <= _at + _ASIZE) => C; last smt().
+   have ?: 0 <= _at < _r8 by smt().
+   have: lastlen <= _ASIZE; last smt().
+   rewrite /lastlen C /=; case: (_ASIZE < _r8) => ?; last smt().
+   have ->: _at + _ASIZE = _r8 + _ASIZE + _at - _r8 by ring.
+   by rewrite -!addzA modzDl !addzA modz_small /#.
+  split; first smt().
+  by apply (stavx2INV_pabsorb _ _ _ H).
+ move => ?????? [st' at' off'] /= Est' Eat' Eoff'.
+ move: H; rewrite /pabsorb_spec_avx2 /absorb_spec_avx2 => [[? H]].
+ rewrite Est' H /addstate_avx2 !stavx2_from_st25K.
+ rewrite /lastpos /niters /lastlen /ABSORB1600 /PABSORB1600 /stateabsorb_last /stateabsorb -cats1; congr; congr.
+ rewrite -addstateA; congr.
+  by congr; rewrite chunk_cat_buf 1:// /#.
+ by rewrite chunkremains_cat_buf /#.
+rcondf 2.
+ by call (:true ==> true) => //.
+ecall (addstate_avx2_h st buf offset _LEN _TRAILB aT).
+auto => |> &m H.
+split.
+ split; first smt(). 
+ split; rewrite /lastlen.
+  case: (_r8 <= _at + _ASIZE) => C; last smt().
+  have ?: 0 <= _at < _r8 by smt().
+  have: lastlen <= _ASIZE; last smt().
+  rewrite /lastlen C /=; case: (_ASIZE < _r8) => ?; last smt().
+  have ->: _at + _ASIZE = _r8 + _ASIZE + _at - _r8 by ring.
+  by rewrite -!addzA modzDl !addzA modz_small /#.
+ split; first smt().
+ by apply (stavx2INV_pabsorb _ _ _ H).
+move => ????? [st' at' off'] /= Est' Eat' Eoff'.
+split.
+ move: H; rewrite /pabsorb_spec_avx2 => [[? H]]; split; first smt().
+ rewrite Est' H /addstate_avx2 stavx2_from_st25K; congr.
+ rewrite /PABSORB1600 /stateabsorb -addstateA; congr.
+  by rewrite chunk_cat_buf /#.
+ rewrite -chunkremains_cat_buf 1:/#.
+ by rewrite -nseq1 bytes2state_zext.
+rewrite Eat' b2i0 /lastlen /_at /=.
+case: ( _r8 <= size _l %% _r8 + _ASIZE ) => C /=.
+ by rewrite /_at modzDml.
+by rewrite eq_sym -modzDml modz_small /#.
+qed.
 
 phoare absorb_avx2_ph _l _buf _tb _r8:
  [ MM.__absorb_avx2
  : aT = size _l %% _r8 /\ buf=_buf /\ _RATE8=_r8 /\ _TRAILB=_tb
  /\ pabsorb_spec_avx2 _r8 _l st
+ /\ 0 <= _tb < 256 /\ 0 < _r8
  ==> if _tb <> 0
      then absorb_spec_avx2 _r8 _tb (_l ++ to_list _buf) res.`1
      else pabsorb_spec_avx2 _r8 (_l ++ to_list _buf) res.`1
