proof/amd64/common/Keccak1600_subreadwrite.ec
@@ -1,19 +1,90 @@
-require import AllCore IntDiv CoreMap List Distr.
+require import AllCore IntDiv List StdOrder.
 
 from Jasmin require import JModel_x86.
+from CryptoSpecs require import Keccak1600_Spec.
 from JazzEC require import Keccak1600_Jazz.
 
 import SLH64.
+import IntOrder.
 
+lemma u64_shl0 (w: W64.t): w `<<<` 0 = w.
+proof. by apply W64.wordP => i Hi; rewrite shlwE Hi /=. qed.
 
 lemma SHLQ_ll: islossless M.__SHLQ
 by islossless.
 
+hoare SHLQ_h _w _sh:
+ M.__SHLQ
+ : x = _w /\ shbytes = _sh /\ 0 <= _sh < 8
+ ==> res = _w `<<<` (8*_sh).
+proof.
+proc; simplify.
+if => //.
+ auto => /> *.
+ by rewrite /W64.(`<<`) of_uintK modz_small /#.
+by auto => /> *; rewrite u64_shl0.
+qed.
+
+phoare SHLQ_ph _w _sh:
+ [ M.__SHLQ
+ : x = _w /\ shbytes = _sh /\ 0 <= _sh < 8
+ ==> res = _w `<<<` (8*_sh)
+ ] = 1%r.
+proof. by conseq SHLQ_ll (SHLQ_h _w _sh). qed.
+
 lemma SHLDQ_ll: islossless M.__SHLDQ
 by islossless.
 
+hoare SHLDQ_h _w _sh:
+ M.__SHLDQ
+ : x = _w /\ shbytes = _sh /\ 0 <= _sh < 16
+ ==> res = _w `<<<` (8*_sh).
+proof.
+proc; simplify.
+if => //.
+ auto => /> *.
+ by rewrite /VPSLLDQ_128 of_uintK modz_small /#.
+auto => /> *; apply W128.wordP => i Hi.
+by rewrite shlwE Hi /=.
+qed.
+
+phoare SHLDQ_ph _w _sh:
+ [ M.__SHLDQ
+ : x = _w /\ shbytes = _sh /\ 0 <= _sh < 16
+ ==> res = _w `<<<` (8*_sh)
+ ] = 1%r.
+proof. by conseq SHLDQ_ll (SHLDQ_h _w _sh). qed.
+
 lemma SHLQ_256_ll: islossless M.__SHLQ_256
 by islossless.
+
+hoare SHLQ_256_h _w _sh:
+ M.__SHLQ_256
+ : x = _w /\ shbytes = _sh /\ 0 <= _sh < 16
+ ==> res = W4u64.pack4 [ (_w \bits64 0) `<<<` (8*_sh)
+                       ; (_w \bits64 1) `<<<` (8*_sh)
+                       ; (_w \bits64 2) `<<<` (8*_sh)
+                       ; (_w \bits64 3) `<<<` (8*_sh)
+                       ].
+proof.
+proc; simplify.
+if => //.
+ auto => /> *.
+ by rewrite /VPSLL_4u64 of_uintK modz_small /#.
+by auto => /> *; rewrite !u64_shl0 pack4E /= -all_eqP /all_eq /=.
+qed.
+
+phoare SHLQ_256_ph _w _sh:
+ [ M.__SHLQ_256
+ : x = _w /\ shbytes = _sh /\ 0 <= _sh < 16
+ ==> res = W4u64.pack4 [ (_w \bits64 0) `<<<` (8*_sh)
+                       ; (_w \bits64 1) `<<<` (8*_sh)
+                       ; (_w \bits64 2) `<<<` (8*_sh)
+                       ; (_w \bits64 3) `<<<` (8*_sh)
+                       ]
+ ] = 1%r.
+proof. by conseq SHLQ_256_ll (SHLQ_256_h _w _sh). qed.
+
 
 lemma m_ilen_read_upto8_at_ll: islossless M.__m_ilen_read_upto8_at
 by islossless.
@@ -530,12 +601,12 @@ op subread_pre cur at len tb =
  && at+len+b2i (tb<>0) <= 200
  && (cur<=at || len=0 && tb=0).
 
-op wat size cur at l=
+op bytes_at size cur at l=
  take size (drop cur (nseq at W8.zero++l)++nseq size W8.zero).
 
-lemma size_wat sz cur at l:
+lemma size_bytes_at sz cur at l:
  0 <= sz =>
- size (wat sz cur at l) = sz.
+ size (bytes_at sz cur at l) = sz.
 proof.
 move=> Hsz; rewrite size_take // size_cat size_nseq.
 smt(size_ge0).
@@ -545,17 +616,17 @@ lemma sub0 (buf: W8.t A.t) off:
  sub buf off 0 = [].
 proof. by rewrite -size_eq0 size_sub /#. qed.
 
-lemma nth_wat sz cur at buf off len tb i:
+lemma nth_bytes_at sz cur at buf off len tb i:
  0 <= sz =>
  subread_pre cur at len tb =>
- nth W8.zero (wat sz cur at (A.sub buf off len++[W8.of_int tb])) i
+ nth W8.zero (bytes_at sz cur at (A.sub buf off len++[W8.of_int tb])) i
  = if 0 <= at-cur <= i < sz
    then nth W8.zero (sub buf off len++[W8.of_int tb]) (cur+i-at)
    else W8.zero.
 proof.
 move=> /> ???????[H|H].
 + case: (0 <= i < sz) => C; last first.
-   by rewrite nth_out 1:size_wat // ifF /#.
+   by rewrite nth_out 1:size_bytes_at // ifF /#.
   case: (i < at-cur) => C1.
    rewrite ifF 1:/# nth_take 1..2:/# nth_cat ifT.
     by rewrite size_drop // !size_cat size_sub //= size_nseq /#.
@@ -567,7 +638,7 @@ move=> /> ???????[H|H].
    by rewrite ifT 1:/# nth_drop 1..2:/# nth_cat size_nseq ifF /#.
   rewrite ifF 1:/# nth_nseq 1:/# nth_out //.
   by rewrite size_cat size_sub /#.
-move=> []->->; rewrite sub0 /= /wat.
+move=> []->->; rewrite sub0 /= /bytes_at.
 case: (0 <= i < sz) => C; last first.
  rewrite nth_out // size_take // size_cat.
  by rewrite size_drop // size_cat !size_nseq /#.
@@ -587,16 +658,182 @@ op subread_spec
  0 <= size =>
  subread_pre cur at len tb =>
  subread_pre (cur+size) at' len' tb'
- /\ w = wat size cur at (sub buf (off+dlt) len ++ [W8.of_int tb])
+ /\ w = bytes_at size cur at (sub buf (off+dlt) len ++ [W8.of_int tb])
  /\ at+len+b2i(tb<>0)=at'+len'+b2i(tb'<>0)
  /\ (tb'=tb || len'=0 && tb'=0)
  /\ dlt+len = dlt'+len'
  /\ at' = max at
               (min (cur+size)
                    (at+len+b2i (tb<>0)))
- /\ len' = max 0 (len - (min 0 (cur+size-at)))
+ /\ len' = max 0 (len - (max 0 (cur+size-at)))
  .
 
+lemma subread_specP N buf off dlt len trail cur at dlt' at' w':
+ 0 <= N =>
+ cur <= at =>
+ subread_pre cur at len trail =>
+ subread_spec N buf off dlt len trail cur at dlt' 0 0 at' w' =>
+ at' = at + len + b2i (trail%%256<>0)
+ /\
+ dlt' = dlt + len
+ /\
+ bytes2state (nseq at W8.zero ++ sub buf (off+dlt) len ++ [W8.of_int trail])
+ = bytes2state (nseq cur W8.zero++w').
+proof.
+move=> Hn Hcur Hpre Hspec.
+move: (Hpre) (Hspec Hn Hpre) => {Hspec} /> ???? H1 H2 H3 H4 H5.
+rewrite !b2i0 /= => H6 H7 H8.
+split; first smt().
+rewrite tP => i Hi.
+rewrite !initiE //= !nth_w64L_from_bytes 1..2:/#.
+congr; apply W8u8.Pack.ext_eq => k Hk.
+rewrite !get_of_list //.
+rewrite eq_sym !nth_take 1..4:/# !nth_drop 1..4:/# -catA nth_cat 1:size_nseq ?Eat.
+case: (8 * i + k < max 0 cur) => Ccur //.
+ rewrite nth_cat ?size_nseq ifT 1:/#.
+ by rewrite !nth_nseq_if /#.
+rewrite eq_sym nth_cat size_nseq /=.
+case: (8*i+k < max 0 at) => C1.
+ by rewrite nth_nseq_if nth_bytes_at /#.
+have ->: max 0 at = at by smt().
+have ->: max 0 cur = cur by smt().
+case: (len=0) => C2.
+ by rewrite C2 nth_bytes_at 1..2:/# sub0 /#.
+rewrite nth_bytes_at 1:/# 1:/#.
+case: (0 <= at - cur <= 8 * i + k - cur < N) => ?.
+ smt().
+rewrite nth_cat ?size_sub 1:/#.
+case: (8 * i + k - at < len) => ? //.
+ by rewrite nth_out /#.
+smt().
+qed.
+
+lemma subread_spec_ahead8 _buf _off _dlt _len _tb _cur _at:
+ _cur + 8 <= _at =>
+ subread_spec 8 _buf _off _dlt _len _tb _cur _at _dlt _len _tb _at (u64bytes W64.zero).
+proof.
+move => H; rewrite /subread_spec => _ Hpre; split; first by smt().
+split; last smt().
+apply (eq_from_nth W8.zero); rewrite size_to_list.
+ by rewrite size_bytes_at /#.
+move=> i Hi; rewrite nth_bytes_at // ifF 1:/#.
+by rewrite nth_to_list W8u8.get_zero.
+qed.
+
+lemma subread_spec_ahead32 _buf _off _dlt _len _tb _cur _at:
+ _cur + 32 <= _at =>
+ subread_spec 32 _buf _off _dlt _len _tb _cur _at _dlt _len _tb _at (u256bytes W256.zero).
+proof.
+move => H; rewrite /subread_spec => _ Hpre; split; first by smt().
+split; last smt().
+apply (eq_from_nth W8.zero); rewrite size_to_list.
+ by rewrite size_bytes_at /#.
+move=> i Hi; rewrite nth_bytes_at 1..2:/# ifF 1:/#.
+by rewrite nth_to_list W32u8.get_zero.
+qed.
+
+lemma subread_spec_empty8 _buf _off _dlt _len _tb _cur _at:
+ _len <= 0 /\ _tb = 0 =>
+ subread_spec 8 _buf _off _dlt _len _tb _cur _at _dlt _len _tb _at (u64bytes W64.zero).
+proof.
+move => [Hlen ->]; rewrite /subread_spec /u64bytes /= !b2i0 /= => Hpre; split; first by smt().
+have ->: _len=0 by smt().
+split; last smt().
+apply (eq_from_nth W8.zero).
+ rewrite size_bytes_at /#.
+move=> i Hi; rewrite nth_bytes_at 1..2:/# !W8u8.get_zero /=.
+case: (0 <= _at - _cur <= i < 8) => C//.
+by rewrite nth_cat ?size_sub 1:/# sub0 /=.
+qed.
+
+lemma subread_spec_empty32 _buf _off _dlt _len _tb _cur _at:
+ _len <= 0 /\ _tb = 0 =>
+ subread_spec 32 _buf _off _dlt _len _tb _cur _at _dlt _len _tb _at (u256bytes W256.zero).
+proof.
+move => [Hlen ->]; rewrite /subread_spec /u256bytes /= !b2i0 /= => Hpre; split; first by smt().
+have ->: _len=0 by smt().
+split; last smt().
+apply (eq_from_nth W8.zero).
+ by rewrite size_bytes_at /#.
+move=> i Hi; rewrite nth_bytes_at 1..2:/# !W32u8.get_zero /=.
+case: (0 <= _at - _cur <= i < 32) => C//.
+by rewrite nth_cat ?size_sub 1:/# sub0 /=.
+qed.
+
+(*
+lemma subread_spec_finished N buf off dlt cur at:
+ at < cur =>
+ subread_spec N buf 
+*)
+
+lemma bytes_at_absorb _buf _off _len _tb _at:
+ 0 <= _len => 0 <= _at =>
+ bytes2state (nseq _at W8.zero ++ A.sub _buf _off _len ++ [W8.of_int _tb]) =
+ bytes2state (bytes_at 200 0 _at (sub _buf _off _len ++ [W8.of_int _tb])).
+proof.
+move => *.
+rewrite /bytes_at drop0 /_statebytes -!bytes2stbytesP.
+apply stbytes_inj.
+rewrite !stwordsK tP => i Hi.
+rewrite !get_of_list 1..2:// nth_take 1..2:/# eq_sym nth_cat.
+rewrite !size_cat !size_nseq !size_sub 1:/# /= lez_maxr 1:/# addzA catA.
+case: (i < _at + _len+1) => C//.
+ rewrite eq_sym nth_out.
+ by rewrite !size_cat !size_nseq !size_sub 1:/# /= lez_maxr 1:/# /#.
+by rewrite nth_nseq 1:/#.
+qed.
+
+
+lemma subread_full buf off len tb at dlt' len' tb' at' wl:
+ subread_pre 0 at len tb => 
+ subread_spec 200 buf off 0 len tb 0 at dlt' len' tb' at' wl =>
+ at+len+b2i (tb<>0) <= 200 =>
+ len' = 0 /\ tb' = 0
+ /\ at'=at+len+b2i(tb<>0) /\ dlt'=len
+ /\ bytes2state (u8zeros at ++ sub buf off len ++ [W8.of_int tb])
+    = bytes2state wl.
+proof.
+move=> Hpre Hspec.
+move: (Hspec _ Hpre) => //.
+move: Hpre => /= Hpre [#] Hpre' -> /= *.
+do (split; first smt()).
+by rewrite bytes_at_absorb 1..2:/#.
+qed.
+
+
+lemma subread_finished size buf off len tb at dlt' len' tb' at' wl:
+ 0 <= size =>
+ subread_pre 0 at len tb => 
+ subread_spec size buf off 0 len tb 0 at dlt' len' tb' at' wl =>
+ len' = 0 =>
+ tb' = 0 =>
+ at'= max at (at+len+b2i(tb<>0)) /\ dlt'=len
+ /\ bytes2state (u8zeros at ++ sub buf off len ++ [W8.of_int tb])
+    = bytes2state wl.
+proof.
+move=> Hsize Hpre Hspec Hlen' Htb'.
+move: (Hspec Hsize Hpre).
+move: Hpre => /= Hpre [#] Hpre' -> /= *.
+do (split; first smt()).
+case: (len=0 /\ tb=0) => C.
+ rewrite -!bytes2stbytesP; apply stbytes_inj; rewrite !stwordsK tP => i Hi.
+ rewrite !get_of_list 1..2:// nth_bytes_at 1..2:/#.
+ by move: C => [-> ->]; rewrite sub0 cats0 /= -nseq1 cat_nseq 1..2:/# nth_nseq_if /#.
+have: at+len+b2i(tb<>0) <= size by smt().
+move=> C'.
+rewrite -!bytes2stbytesP; apply stbytes_inj; rewrite !stwordsK tP => i Hi.
+rewrite !get_of_list 1..2:// nth_bytes_at 1..2:/# /=.
+case: (0 <= at <= i < size) => Ci.
+ by rewrite -!catA nth_cat size_nseq ifF /#.
+move: Ci. rewrite andaE negb_and (:0 <= at) 1:/# /= => [[Ci1|Ci2]].
+ by rewrite -catA nth_cat size_nseq ifT 1:/# nth_nseq_if /#.
+rewrite nth_cat size_cat size_nseq size_sub 1:/# ifF 1:/#.
+case: (tb=0) => Ctb.
+ by rewrite Ctb /#.
+by rewrite ifF /#.
+qed.
+
+(*
 lemma subread_finish R size buf off dlt len tb cur at dlt' len' tb' at' wl:
  0 <= size =>
  subread_pre cur at len tb => 
@@ -611,6 +848,10 @@ move: (Hspec Hsize Hpre).
 move: {Hspec} Hpre => /> ??? Hinv Hend _ _ ?? Hat HH.
 by move=> H1 H2 /#.
 qed.
+*)
+
+require import StdOrder.
+import IntOrder.
 
 lemma subread_spec_cat N1 N2 buf off dlt dlt' dlt'' len len' len'' tb tb' tb'' cur at at' at'' w' w'':
  0 <= N1 => 0 <= N2 =>
@@ -624,14 +865,14 @@ move: (H2 HN2 Hpre2) => []Hpre3 {H2} [#]->*.
 split; first smt().
 split; last smt().
 apply (eq_from_nth W8.zero).
- by rewrite size_cat !size_wat /#.
-rewrite size_cat !size_wat 1..2:/# => i Hi.
-rewrite nth_cat size_wat 1:/#.
+ by rewrite size_cat !size_bytes_at /#.
+rewrite size_cat !size_bytes_at 1..2:/# => i Hi.
+rewrite nth_cat size_bytes_at 1:/#.
 case: (i<N1) => Ci.
- by rewrite !nth_wat /#.
+ by rewrite !nth_bytes_at /#.
 case: (at<cur) => Hcur.
- by rewrite !nth_wat /#.
-rewrite !nth_wat 1..4:/#.
+ by rewrite !nth_bytes_at /#.
+rewrite !nth_bytes_at 1..4:/#.
 rewrite (:cur+N1+(i-N1)-at'=cur+i-at') 1:/#.
 case: (at'<cur+N1) => Cat'.
  have ->: len'=0 by smt().
@@ -641,32 +882,75 @@ case: (at'<cur+N1) => Cat'.
  by rewrite nth_out // size_cat size_sub /#.
 case: (at<=cur+N1) => Cat.
  rewrite ifT 1:/# ifT 1:/#.
- have ->: at'=cur+N1 by smt().
- case: (tb'=tb) => Ctb; first smt().
+ have : at'=cur+N1 by smt().
+ move => />.
+ case: (tb'=tb) => Ctb.
+  rewrite nth_cat ?size_sub 1:/#.
+  case: (cur + i - (cur + N1) < len - (cur + N1 - at)) => CC.
+   by rewrite nth_sub 1:/# nth_cat ?size_sub 1:/# ifT 1:/# nth_sub 1:/# /#.
+  case: (tb=0) => Etb.
+   by rewrite nth_cat ?size_sub 1:/# ifF 1:/# /#.
+  rewrite nth_cat ?size_sub 1:/#.
+  case: (cur + i - at < len) => ?.
+   by rewrite nth_sub /#.
+  smt().
  have ->: len'=0 by smt().
  have ->: tb'=0 by smt().
- have ?: len < cur-at+N1 by smt().
  rewrite sub0 /= nth_cat size_sub 1:/#.
  by rewrite ifF 1:/# nth_out /#.
 smt().
 qed.
 
-
-op u64_to_bytes w = W8u8.to_list w.
-op u128_to_bytes w = W16u8.to_list w.
-op u256_to_bytes w = W32u8.to_list w.
-
+lemma bytes_at8_zero cur at:
+ 0 <= cur =>
+ bytes_at 8 cur at [W8.zero] = u64bytes W64.zero.
+proof.
+move=> *.
+rewrite /bytes_at; apply (eq_from_nth W8.zero).
+ by rewrite size_to_list size_take 1:/# !size_cat size_drop 1:/# size_cat !size_nseq /= /#.
+rewrite size_take 1:/# !size_cat size_drop 1:/# size_cat !size_nseq /=.
+move=> i Hi.
+rewrite nth_take 1..2:/# nth_cat ?size_drop 1:/# u64bytes0 nth_drop 1..2:/# nth_cat !nth_u8zeros /#.
+qed.
 
 hoare a_ilen_read_upto8_at_h _buf _off _dlt _len _trail _cur _at:
  MM.__a_ilen_read_upto8_at
  : buf=_buf /\ offset=_off /\ dELTA=_dlt /\ lEN=_len /\ tRAIL=_trail /\ cUR=_cur /\ aT=_at
- ==> subread_spec 8 _buf _off _dlt _len _trail _cur _at res.`1 res.`2 res.`3 res.`4 (u64_to_bytes res.`5).
-admitted.
+ ==> subread_spec 8 _buf _off _dlt _len _trail _cur _at res.`1 res.`2 res.`3 res.`4 (u64bytes res.`5).
+proof.
+proc; simplify.
+if => //.
+ auto => /> [[H|H]|H].
+ + move=> _; rewrite /subread_pre => /> ??????.
+   rewrite (:!_cur<=_at) 1:/# /= => [[Elen Etb]].
+   rewrite !Elen !Etb; split; first smt().
+   split.
+    rewrite sub0 bytes_at8_zero /#. 
+   smt().
+  + apply subread_spec_ahead8; smt().
+  apply subread_spec_empty8; smt().
+sp; if => //.
+ (* 8 <= lEN *)
+ wp; ecall (SHLQ_h w aT8); auto => /> *.
+ split; first smt().
+ move=> *; split; first smt().
+ split.
+  admit.
+ smt().
+(* subread *)
+if => //=.
+ (* 4 <= lEN *)
+ admit.
+(* lEN < 4 *)
+admit.
+qed.
+
+
 
 phoare a_ilen_read_upto8_at_ph _buf _off _dlt _len _trail _cur _at:
  [ MM.__a_ilen_read_upto8_at
  : buf=_buf /\ offset=_off /\ dELTA=_dlt /\ lEN=_len /\ tRAIL=_trail /\ cUR=_cur /\ aT=_at
- ==> subread_spec 8 _buf _off _dlt _len _trail _cur _at res.`1 res.`2 res.`3 res.`4 (u64_to_bytes res.`5)
+ ==> subread_spec 8 _buf _off _dlt _len _trail _cur _at res.`1 res.`2 res.`3 res.`4 (u64bytes res.`5)
  ] = 1%r.
 proof.
 by conseq a_ilen_read_upto8_at_ll
@@ -676,13 +960,13 @@ qed.
 hoare a_ilen_read_upto16_at_h _buf _off _dlt _len _trail _cur _at:
  MM.__a_ilen_read_upto16_at
  : buf=_buf /\ offset=_off /\ dELTA=_dlt /\ lEN=_len /\ tRAIL=_trail /\ cUR=_cur /\ aT=_at
- ==> subread_spec 16 _buf _off _dlt _len _trail _cur _at res.`1 res.`2 res.`3 res.`4 (u128_to_bytes res.`5).
+ ==> subread_spec 16 _buf _off _dlt _len _trail _cur _at res.`1 res.`2 res.`3 res.`4 (u128bytes res.`5).
 admitted.
 
 phoare a_ilen_read_upto16_at_ph _buf _off _dlt _len _trail _cur _at:
  [ MM.__a_ilen_read_upto16_at
  : buf=_buf /\ offset=_off /\ dELTA=_dlt /\ lEN=_len /\ tRAIL=_trail /\ cUR=_cur /\ aT=_at
- ==> subread_spec 16 _buf _off _dlt _len _trail _cur _at res.`1 res.`2 res.`3 res.`4 (u128_to_bytes res.`5)
+ ==> subread_spec 16 _buf _off _dlt _len _trail _cur _at res.`1 res.`2 res.`3 res.`4 (u128bytes res.`5)
  ] = 1%r.
 proof.
 by conseq a_ilen_read_upto16_at_ll
@@ -692,19 +976,49 @@ qed.
 hoare a_ilen_read_upto32_at_h _buf _off _dlt _len _trail _cur _at:
  MM.__a_ilen_read_upto32_at
  : buf=_buf /\ offset=_off /\ dELTA=_dlt /\ lEN=_len /\ tRAIL=_trail /\ cUR=_cur /\ aT=_at
- ==> subread_spec 32 _buf _off _dlt _len _trail _cur _at res.`1 res.`2 res.`3 res.`4 (u256_to_bytes res.`5).
+ ==> subread_spec 32 _buf _off _dlt _len _trail _cur _at res.`1 res.`2 res.`3 res.`4 (u256bytes res.`5).
 admitted.
 
 phoare a_ilen_read_upto32_at_ph _buf _off _dlt _len _trail _cur _at:
  [ MM.__a_ilen_read_upto32_at
  : buf=_buf /\ offset=_off /\ dELTA=_dlt /\ lEN=_len /\ tRAIL=_trail /\ cUR=_cur /\ aT=_at
- ==> subread_spec 32 _buf _off _dlt _len _trail _cur _at res.`1 res.`2 res.`3 res.`4 (u256_to_bytes res.`5)
+ ==> subread_spec 32 _buf _off _dlt _len _trail _cur _at res.`1 res.`2 res.`3 res.`4 (u256bytes res.`5)
  ] = 1%r.
 proof.
 by conseq a_ilen_read_upto32_at_ll
           (a_ilen_read_upto32_at_h _buf _off _dlt _len _trail _cur _at).
 qed.
 
+require import Keccak_bindings.
 
+lemma trunc_zext_u64_u128 w:
+ truncateu64 (W2u64.zeroextu128 w) = w.
+proof.
+rewrite zeroextu128E /truncateu64.
+admitted.
+
+equiv a_ilen_read_bcast_upto8_at_eq:
+ MM.__a_ilen_read_bcast_upto8_at
+ ~ MM.__a_ilen_read_upto8_at
+ : ={arg}
+ ==> (res.`1,res.`2,res.`3,res.`4,res.`5){1}
+     = (res.`1,res.`2,res.`3,res.`4,VPBROADCAST_4u64 (truncateu64 (zeroextu128 res.`5))){2}.
+proof.
+proc; simplify.
+if => //=.
+ auto => />.
+ by move=> *; clear; circuit.
+sp; if => //=.
+ inline*; auto => /> &m *; split => *.
+  rewrite /VPSLL_4u64 /VPBROADCAST_4u64 /= -iotaredE /=; congr; congr=> />.
+  (do split);
+  (rewrite /W64.(`<<`) trunc_zext_u64_u128; congr;
+   [ congr; admit
+   | rewrite of_uintK modz_small 1:/# of_uintK modz_small /#]).
+  rewrite /W64.(`<<`) trunc_zext_u64_u128; congr; congr; admit.
+inline *.
+rcondf {1} 9; first by auto.
+rcondf {1} 10; first by auto.
+admitted.
 
 end ReadWriteArray.
